examples/seplogic/SepLogic.Heap.fst
@@ -1,8 +1,5 @@
 module SepLogic.Heap
 
-module S  = FStar.Set
-module TS = FStar.TSet
-
 private noeq type heap_rec = {
   next_addr: nat;
   memory   : nat -> Tot (option (a:Type0 & a))
@@ -10,245 +7,135 @@ private noeq type heap_rec = {
 
 let heap = h:heap_rec{(forall (n:nat). n >= h.next_addr ==> None? (h.memory n))}
 
+private let equal_heaps (h0 h1:heap) =
+  let _ = () in
+  h0.next_addr = h1.next_addr /\
+  FStar.FunctionalExtensionality.feq h0.memory h1.memory
+
+private let equal_heaps_extensional (h0 h1:heap)
+  : Lemma (requires True) (ensures (equal_heaps h0 h1 <==> h0 == h1))
+  = ()
+  
+let memory = nat -> Tot (option (a:Type0 & a))
+
+private let equal_memories (m0 m1:memory) =
+  let _ = () in
+  FStar.FunctionalExtensionality.feq m0 m1
+
+private let equal_memories_extensional (m0 m1:memory)
+  : Lemma (requires True) (ensures (equal_memories m0 m1 <==> m0 == m1))
+  = ()
+
+let emp = fun _ -> None
+
 let ref a = nat
 
 let addr_of #a n = n
 
-private let equal (h1 h2:heap) =
+let heap_memory h = h.memory
+
+let disjoint_heaps h0 h1 =
   let _ = () in
-  h1.next_addr = h2.next_addr /\
-  FStar.FunctionalExtensionality.feq h1.memory h2.memory
+  (forall r . ~(Some?(h0.memory r) && Some?(h1.memory r)))
 
-private let equal_extensional (h0 h1:heap)
-  : Lemma (requires True) (ensures (equal h0 h1 <==> h0 == h1))
-  = ()
+let disjoint_memories m0 m1 =
+  let _ = () in
+  (forall r . ~(Some?(m0 r) && Some?(m1 r)))
 
-let emp = fun h -> h.next_addr = 0 /\ (forall r . None? (h.memory r))
+let disjoint_heaps_comm h0 h1 = ()
 
-let join_tot h0 h1 =
+let disjoint_memories_emp m = ()
+
+let disjoint_memories_comm m0 m1 = ()
+
+let disjoint_heaps_memories h0 h1 = ()
+
+let join h0 h1 = 
   let memory = (fun r' ->  match (h0.memory r', h1.memory r') with
                               | (Some v1, None) -> Some v1
 			      | (None, Some v2) -> Some v2
-			      | _               -> None) in
+			      | (None, None)    -> None) in
   if (h0.next_addr < h1.next_addr)
   then { next_addr = h1.next_addr; memory = memory }
   else { next_addr = h0.next_addr; memory = memory }
 
-private let join_tot_comm' (h0 h1:heap)
-  : Lemma (equal (join_tot h0 h1) (join_tot h1 h0))
-  = ()
-
-let join_tot_comm h0 h1
-  = join_tot_comm' h0 h1
-
-let disjoint #a #b r0 r1 = r0 =!= r1
-
-let disjoint_comm #a #b r0 r1 = ()
-
-let disjoint_heaps h0 h1 =
-  let _ = () in
-  (forall (r:nat). ~(Some?(h0.memory r) && Some?(h1.memory r)))
-
-let disjoint_heaps_emp h0 h1 = ()
-
-let disjoint_heaps_comm h0 h1 = ()
-
-private let init_heap : heap = 
-  let memory = fun r -> None in
-  {next_addr = 0; memory = memory}
-
-private let lemma_init_heap_emp ()
-  : Lemma (emp (init_heap))
-  = ()
+let join_comm h0 h1 = assert (equal_heaps (join h0 h1) (join h1 h0))
 
 let ( |> ) #a r x = 
-  fun h -> h.memory r == Some (| a , x |) /\ (forall r' . r =!= r' ==> None? (h.memory r'))  
+  fun r' -> if r = r' then Some (| a , x |)
+                      else None
 
-let ( <*> ) p q = 
-  fun h -> exists h0 h1 . disjoint_heaps h0 h1 /\ h == join_tot h0 h1 /\ p h0 /\ q h1 
+let ( <*> ) m0 m1 = 
+  fun r -> match (m0 r, m1 r) with
+           | (Some v1, None) -> Some v1
+           | (None, Some v2) -> Some v2
+           | (None, None)    -> None
 
-let sep_interp p q h = 
-  assert_norm ((p <*> q) h ==> (exists h0 h1 . disjoint_heaps h0 h1 /\ h == join_tot h0 h1 /\ p h0 /\ (q h1)))
+let sep_join h0 h1 = 
+  assert (equal_memories (heap_memory (join h0 h1)) 
+                         ((heap_memory h0) <*> (heap_memory h1)))
 
-private let lemma_join_tot_emp' (h0 h1:heap)
-  : Lemma (emp h1 ==> equal (join_tot h0 h1) h0)
-  = ()
+let split_heap m0 m1 h = 
+  let h0 = { next_addr = h.next_addr; memory = m0 } in
+  let h1 = { next_addr = h.next_addr; memory = m1 } in
+  (h0,h1)
 
-private let lemma_join_tot_emp (h0 h1:heap)
-  : Lemma (emp h1 ==> (join_tot h0 h1) == h0)
-          [SMTPat (join_tot h0 h1); 
-           SMTPat (emp h1)]
-  = lemma_join_tot_emp' h0 h1
+let split_heap_disjoint m0 m1 h = ()
 
-private let sep_emp'  (p:hpred) (h:heap) (h0 h1:heap)
-  : Lemma ((disjoint_heaps h0 h1 /\ h == join_tot h0 h1 /\ p h0 /\ (emp h1)) ==> p h)
-  = lemma_join_tot_emp h0 h1
+let split_heap_join m0 m1 h = 
+  assert (let (h0,h1) = split_heap m0 m1 h in
+          equal_heaps h (join h0 h1))
 
-let sep_emp p h = 
-  sep_interp p emp h;
-  FStar.Classical.forall_to_exists (fun h1 -> FStar.Classical.forall_to_exists (fun h0 -> sep_emp' p h h0 h1));
-  FStar.Classical.move_requires (fun h -> 
-    FStar.Classical.exists_intro (fun h1 -> exists h0 . disjoint_heaps h0 h1 /\ h == join_tot h0 h1 /\ p h0 /\ (emp h1)) init_heap) h
-  
-private let lemma_sep_comm (p q:hpred) (h h0 h1:heap)
-  : Lemma ((disjoint_heaps h0 h1 /\ h == join_tot h0 h1 /\ p h0 /\ q h1) 
-           ==> 
-           (exists h0 h1 . disjoint_heaps h1 h0 /\ h == join_tot h1 h0 /\ p h0 /\ q h1))
-  = join_tot_comm h0 h1
+let split_heap_memories m0 m1 h = ()
 
-private let lemma_sep_comm' (p q:hpred) (h:heap)
-  : Lemma ((exists h0 h1 . disjoint_heaps h0 h1 /\ h == join_tot h0 h1 /\ p h0 /\ q h1) 
-           ==> 
-           (exists h0 h1 . disjoint_heaps h1 h0 /\ h == join_tot h1 h0 /\ p h0 /\ q h1))
-  = FStar.Classical.forall_to_exists (fun h1 -> FStar.Classical.forall_to_exists (fun h0 -> lemma_sep_comm p q h h0 h1))
-
-let sep_comm p q h = lemma_sep_comm' p q h; lemma_sep_comm' q p h
-
-private let lemma_join_tot_assoc' (h0 h1 h2:heap)
-  : Lemma (requires (disjoint_heaps h0 h1 /\ disjoint_heaps h1 h2 /\ disjoint_heaps h0 h2))
-          (ensures  (equal (join_tot h0 (join_tot h1 h2)) (join_tot (join_tot h0 h1) h2)))
-  = ()
-
-private let lemma_join_tot_assoc (h0 h1 h2:heap)
-  : Lemma (requires (disjoint_heaps h0 h1 /\ disjoint_heaps h1 h2 /\ disjoint_heaps h0 h2))
-          (ensures  (join_tot h0 (join_tot h1 h2) == join_tot (join_tot h0 h1) h2))
-          [SMTPat (join_tot h0 (join_tot h1 h2)); 
-           SMTPat (join_tot (join_tot h0 h1) h2)]
-  = lemma_join_tot_assoc' h0 h1 h2
-
-private let exists_intro_4 (#a0:Type) (#a1:Type) (#a2:Type) (#a3:Type) 
-                           (p:(a0 -> a1 -> a2 -> a3 -> Type)) 
-                           (witness0:a0) (witness1:a1) (witness2:a2) (witness3:a3)
-  : Lemma (requires (p witness0 witness1 witness2 witness3))
-          (ensures  (exists x0 x1 x2 x3 . p x0 x1 x2 x3))
-  = ()
-
-private let sep_assoc_l2r' (p q r:hpred) (h h0 h1 h1' h1'':heap)
-  : Lemma ((disjoint_heaps h0 h1 /\ h == join_tot h0 h1 /\ p h0 /\ 
-            disjoint_heaps h1' h1'' /\ h1 == join_tot h1' h1'' /\ q h1' /\ r h1'')
-           ==> 
-          (exists h0 h1 h0' h0'' . 
-             disjoint_heaps h0 h1 /\ h == join_tot h0 h1 /\ 
-             disjoint_heaps h0' h0'' /\ h0 == join_tot h0' h0'' /\ p h0' /\ q h0'' /\ r h1))
-  = FStar.Classical.move_requires (fun h -> 
-      exists_intro_4 (fun h0 h1 h0' h0'' -> 
-        disjoint_heaps h0 h1 /\ h == join_tot h0 h1 /\ 
-          disjoint_heaps h0' h0'' /\ h0 == join_tot h0' h0'' /\ p h0' /\ q h0'' /\ r h1)
-        (join_tot h0 h1') h1'' h0 h1') h
-
-private let forall_to_exists_4 (#a0:Type) (#a1:Type) (#a2:Type) (#a3:Type) 
-                               (#p:(a0 -> a1 -> a2 -> a3 -> Type)) (#r:Type) 
-                               ($f:(x0:a0 -> x1:a1 -> x2:a2 -> x3:a3 -> Lemma (p x0 x1 x2 x3 ==> r)))
-  : Lemma ((exists (x0:a0) (x1:a1) (x2:a2) (x3:a3) . p x0 x1 x2 x3) ==> r)
-  = FStar.Classical.forall_to_exists (fun (x3:a3) -> 
-    FStar.Classical.forall_to_exists (fun (x2:a2) -> 
-    FStar.Classical.forall_to_exists (fun (x1:a1) -> 
-    FStar.Classical.forall_to_exists (fun (x0:a0) -> f x0 x1 x2 x3))))
-
-private let sep_assoc_l2r (p q r:hpred) (h:heap)
-  : Lemma ((p <*> (q <*> r)) h ==> ((p <*> q) <*> r) h)
-  = sep_interp p (q <*> r) h;
-    sep_interp (p <*> q) r h;
-    forall_to_exists_4 (fun h0 h1 h1' h1'' -> sep_assoc_l2r' p q r h h0 h1 h1' h1'')
-    
-private let sep_assoc_r2l' (p q r:hpred) (h h0 h1 h0' h0'':heap)
-  : Lemma ((disjoint_heaps h0 h1 /\ h == join_tot h0 h1 /\ 
-            disjoint_heaps h0' h0'' /\ h0 == join_tot h0' h0'' /\ p h0' /\ q h0'' /\ r h1)
-           ==>
-           (exists h0 h1 h1' h1'' . 
-              disjoint_heaps h0 h1 /\ h == join_tot h0 h1 /\ p h0 /\ 
-              disjoint_heaps h1' h1'' /\ h1 == join_tot h1' h1'' /\ q h1' /\ r h1''))
-  = FStar.Classical.move_requires (fun h -> 
-      exists_intro_4 (fun h0 h1 h1' h1'' -> 
-        disjoint_heaps h0 h1 /\ h == join_tot h0 h1 /\ p h0 /\ 
-          disjoint_heaps h1' h1'' /\ h1 == join_tot h1' h1'' /\ q h1' /\ r h1'')
-        h0' (join_tot h0'' h1) h0'' h1) h
-
-private let sep_assoc_r2l (p q r:hpred) (h:heap)
-  : Lemma (((p <*> q) <*> r) h ==> (p <*> (q <*> r)) h)
-  = sep_interp p (q <*> r) h;
-    forall_to_exists_4 (fun h0 h1 h0' h0'' -> sep_assoc_r2l' p q r h h0 h1 h0' h0'');
-    sep_interp (p <*> q) r h
-    
-let sep_assoc p q r h = 
-  sep_assoc_l2r p q r h;
-  sep_assoc_r2l p q r h
-
-let fresh #a r = fun h -> h.memory r == None
-
-let contains #a h r = 
+let hcontains #a h r = 
   let _ = () in 
   exists x . h.memory r == Some (| a , x |)
 
-let points_to_contains #a r x h = ()
+let mcontains #a m r = 
+  let _ = () in 
+  exists x . m r == Some (| a , x |)
 
-let points_to_ext #a r x y h = ()
+let hcontains_mcontains #a r h = ()
 
-private let points_to_disj' (#a:Type) (#b:Type) (r:ref a) (s:ref b) (x:a) (y:b) (h:heap) (h0:heap) (h1:heap)
-  : Lemma ((disjoint_heaps h0 h1 /\ h == join_tot h0 h1 /\ (r |> x) h0 /\ (s |> y) h1) ==> disjoint r s)
-  = ()
+let points_to_mcontains #a r x = ()
 
-private let points_to_disj'' (#a:Type) (#b:Type) (r:ref a) (s:ref b) (x:a) (y:b) (h:heap) (h0:heap) 
-  : Lemma ((exists h1 . disjoint_heaps h0 h1 /\ h == join_tot h0 h1 /\ (r |> x) h0 /\ (s |> y) h1) ==> disjoint r s)
-  = FStar.Classical.forall_to_exists (fun h1 -> points_to_disj' r s x y h h0 h1)
-
-private let points_to_disj''' (#a:Type) (#b:Type) (r:ref a) (s:ref b) (x:a) (y:b) (h:heap) 
-  : Lemma ((exists h0 h1 . disjoint_heaps h0 h1 /\ h == join_tot h0 h1 /\ (r |> x) h0 /\ (s |> y) h1) ==> disjoint r s)
-  = FStar.Classical.forall_to_exists (fun h0 -> points_to_disj'' r s x y h h0)
-
-let points_to_disj #a #b r s x y h = 
-  sep_interp (r |> x) (s |> y) h;
-  points_to_disj''' r s x y h
-
-let join_tot_contains #a r h0 h1 = ()
-
-let sel_tot #a h r =
+let sel #a h r =
   let Some (| _, x |) = h.memory r in
   x
 
-let upd_tot' (#a:Type0) (h:heap) (r:ref a) (x:a) =
+let upd' (#a:Type0) (h:heap) (r:ref a) (x:a) =
   { h with memory = (fun r' -> if r = r' then Some (| a, x |)
                                          else h.memory r') }
 
-let upd_tot #a h r x = upd_tot' h r x
+let upd #a h r x = upd' h r x
 
 let points_to_sel #a r x h = ()
 
-let points_to_upd #a r x v h = ()
+let points_to_upd #a r x v h = 
+  assert (equal_memories (heap_memory ((upd h r v))) (r |> v))
 
-let restrict #a h r =
-  { next_addr = h.next_addr;
-    memory    = (fun (r':nat) -> if r' = r then h.memory r' else None) }
+let hfresh #a r h = 
+  h.memory r == None
 
-let minus #a h r =
-  { h with memory = (fun (r':nat) -> if r' = r then None else h.memory r') }
+let mfresh #a r m = 
+  m r == None
 
-let minus_not_contains #a r h = ()
+let hfres_mfresh #a r h = ()
 
-let restrict_points_to #a r h = ()
+let alloc #a h0 x = 
+  let r = h0.next_addr in
+  let memory1 = (fun r' -> if r = r' then Some (| a , x |)
+                                     else h0.memory r') in
+  let h1 = { next_addr = h0.next_addr + 1; memory = memory1 } in
+  (r, h1)
 
-let disjoint_heaps_restrict_minus #a r h = ()
+let alloc_fresh #a h0 x = ()
 
-let disjoint_heaps_minus_1 #a r x h = ()
+let alloc_contains #a h0 x = ()
 
-let disjoint_heaps_minus_2 #a r x0 x1 h0 h1 = ()
+let alloc_sel #a h0 x = ()
 
-private let join_tot_restrict_minus' (#a:Type0) (r:ref a) (h:heap)
-  : Lemma (requires (h `contains` r))
-          (ensures  (equal h (join_tot (restrict h r) (minus h r))))
-  = ()
-
-let join_tot_restrict_minus #a r h = 
-  join_tot_restrict_minus' #a r h
-
-private let join_tot_minus_restrict' (#a:Type0) (r:ref a) (h:heap)
-  : Lemma (requires (h `contains` r))
-          (ensures  (equal (join_tot (minus h r) h) (restrict h r)))
-  = ()
-
-let join_tot_minus_restrict #a r h = 
-  join_tot_minus_restrict' r h
-
-let points_to_join_tot_minus #a r x y h h' = ()
-
-let points_to_join_tot_restrict #a r x y h h' = ()
+let alloc_emp_points_to #a h0 x = 
+  assert (let (r,h1) = alloc h0 x in
+          equal_memories (heap_memory h1) (r |> x))
